Change names of inductive constructors.
Prompted by rb_tree, I decided to switch to uppercase names for
constructors. This has the benefit of being more clearly different
from other definitions. The type name of inductive types is still
lowercase in Set/Type and uppercase in Prop.

E1_formula.v
@@ -14,20 +14,20 @@ Variable atom : Type.
 
 (* Basic formula structure. *)
 Inductive wff :=
-  | wff_atom (a : atom)
-  | wff_not (φ : wff)
-  | wff_and (φ ϕ : wff)
-  | wff_ex (φ : wff).
+  | WFF_atom (a : atom)
+  | WFF_not (φ : wff)
+  | WFF_and (φ ϕ : wff)
+  | WFF_ex (φ : wff).
 
 Variable domain : Type.
 Variable Model : atom -> list domain -> Prop.
 
 Fixpoint Realizes (f : wff) (Γ : list domain) :=
   match f with
-  | wff_atom a  => Model a Γ
-  | wff_not φ   => ¬Realizes φ Γ
-  | wff_and φ ϕ => Realizes φ Γ /\ Realizes ϕ Γ
-  | wff_ex φ    => ∃x, Realizes φ (x :: Γ)
+  | WFF_atom a  => Model a Γ
+  | WFF_not φ   => ¬Realizes φ Γ
+  | WFF_and φ ϕ => Realizes φ Γ /\ Realizes ϕ Γ
+  | WFF_ex φ    => ∃x, Realizes φ (x :: Γ)
   end.
 
 Definition Use φ n := ∀Γ, Realizes φ Γ <-> Realizes φ (firstn n Γ).
@@ -35,20 +35,20 @@ Definition Use φ n := ∀Γ, Realizes φ Γ <-> Realizes φ (firstn n Γ).
 Section Facts_about_usage.
 
 Theorem Use_not φ n :
-  Use φ n -> Use (wff_not φ) n.
+  Use φ n -> Use (WFF_not φ) n.
 Proof.
 split; simpl; apply contra, H.
 Qed.
 
 Theorem Use_and φ ϕ n :
-  Use φ n -> Use ϕ n -> Use (wff_and φ ϕ) n.
+  Use φ n -> Use ϕ n -> Use (WFF_and φ ϕ) n.
 Proof.
 intros Hφ Hϕ; split; simpl.
 all: split; [apply (Hφ Γ)|apply (Hϕ Γ)]; apply H.
 Qed.
 
 Theorem Use_ex φ n :
-  Use φ (S n) -> Use (wff_ex φ) n.
+  Use φ (S n) -> Use (WFF_ex φ) n.
 Proof.
 split; simpl; intros [x Hx];
 exists x; now apply (H (x :: Γ)).
@@ -66,17 +66,17 @@ End Facts_about_usage.
 
 End First_order_formulae.
 
-Arguments wff_atom {_}.
-Arguments wff_not {_}.
-Arguments wff_and {_}.
-Arguments wff_ex {_}.
+Arguments WFF_atom {_}.
+Arguments WFF_not {_}.
+Arguments WFF_and {_}.
+Arguments WFF_ex {_}.
 Arguments Realizes {_ _}.
 Arguments Use {_ _}.
 
 Notation model atom domain := (atom -> list domain -> Prop).
-Notation "¬` φ" := (wff_not φ)(right associativity, at level 30, format "¬` φ").
-Notation "φ ∧` ϕ" := (wff_and φ ϕ) (right associativity, at level 35).
-Notation "∃[ φ ]" := (wff_ex φ) (format "∃[ φ ]").
+Notation "¬` φ" := (WFF_not φ)(right associativity, at level 30, format "¬` φ").
+Notation "φ ∧` ϕ" := (WFF_and φ ϕ) (right associativity, at level 35).
+Notation "∃[ φ ]" := (WFF_ex φ) (format "∃[ φ ]").
 Notation "A |= ( φ )[ Γ ]" := (Realizes A φ Γ)
   (at level 20, format "A  |=  ( φ )[ Γ ]").
 
@@ -139,29 +139,29 @@ End Results_about_realization.
 Section Atomic_formulae_for_linear_arithmetic.
 
 Inductive la_term :=
-  | la_zero
-  | la_one
-  | la_var (i : nat)
-  | la_add (x y : la_term).
+  | LA_zero
+  | LA_one
+  | LA_var (i : nat)
+  | LA_add (x y : la_term).
 
 Inductive la_atom :=
-  | la_eq (x y : la_term)
-  | la_le (x y : la_term).
+  | LA_eq (x y : la_term)
+  | LA_le (x y : la_term).
 
 Inductive rel_atom :=
-  | rel_zero (i : nat)
-  | rel_one (i : nat)
-  | rel_add (i j k : nat)
-  | rel_eq (i j : nat)
-  | rel_le (i j : nat).
+  | Rel_zero (i : nat)
+  | Rel_one (i : nat)
+  | Rel_add (i j k : nat)
+  | Rel_eq (i j : nat)
+  | Rel_le (i j : nat).
 
 End Atomic_formulae_for_linear_arithmetic.
 
 Notation formula := (wff la_atom).
 Notation rformula := (wff rel_atom).
 
-Definition formula_atom := @wff_atom la_atom.
-Definition rformula_atom := @wff_atom rel_atom.
+Definition formula_atom := @WFF_atom la_atom.
+Definition rformula_atom := @WFF_atom rel_atom.
 
 Coercion formula_atom : la_atom >-> formula.
 Coercion rformula_atom : rel_atom >-> rformula.
@@ -171,26 +171,26 @@ Section Standard_models_of_linear_arithmetic.
 
 Fixpoint eval (x : la_term) (Γ : list nat) :=
   match x with
-  | la_zero    => 0
-  | la_one     => 1
-  | la_var i   => nth i Γ 0
-  | la_add x y => eval x Γ + eval y Γ
+  | LA_zero    => 0
+  | LA_one     => 1
+  | LA_var i   => nth i Γ 0
+  | LA_add x y => eval x Γ + eval y Γ
   end.
 
 Definition Nat (a : la_atom) (Γ : list nat) :=
   match a with
-  | la_eq x y => eval x Γ = eval y Γ
-  | la_le x y => eval x Γ ≤ eval y Γ
+  | LA_eq x y => eval x Γ = eval y Γ
+  | LA_le x y => eval x Γ ≤ eval y Γ
   end.
 
 Definition NatR (a : rel_atom) (Γ : list nat) :=
   let f := λ i, nth i Γ 0 in
   match a with
-  | rel_zero i    => f i = 0
-  | rel_one i     => f i = 1
-  | rel_add i j k => f i + f j = f k
-  | rel_eq i j    => f i = f j
-  | rel_le i j    => f i ≤ f j
+  | Rel_zero i    => f i = 0
+  | Rel_one i     => f i = 1
+  | Rel_add i j k => f i + f j = f k
+  | Rel_eq i j    => f i = f j
+  | Rel_le i j    => f i ≤ f j
   end.
 
 End Standard_models_of_linear_arithmetic.
@@ -200,13 +200,13 @@ Section Embedding_of_formula_in_rformula.
 
 Fixpoint shift_vars n x :=
   match x with
-  | la_zero    => la_zero
-  | la_one     => la_one
-  | la_var i   => la_var (n + i)
-  | la_add x y => la_add (shift_vars n x) (shift_vars n y)
+  | LA_zero    => LA_zero
+  | LA_one     => LA_one
+  | LA_var i   => LA_var (n + i)
+  | LA_add x y => LA_add (shift_vars n x) (shift_vars n y)
   end.
 
-Notation "# i" := (la_var i) (at level 9, format "# i").
+Notation "# i" := (LA_var i) (at level 9, format "# i").
 Notation "x << n" := (shift_vars n x) (at level 10, format "x << n").
 
 Theorem eval_shift_vars x Γ n :
@@ -219,15 +219,15 @@ induction x; simpl. 1,2: easy.
 Qed.
 
 Lemma reduce_la_term j x n :
-  Σ ϕ, ∀Γ, Nat |= (la_eq #j (x<<n))[Γ] <-> NatR |= (ϕ)[Γ].
+  Σ ϕ, ∀Γ, Nat |= (LA_eq #j (x<<n))[Γ] <-> NatR |= (ϕ)[Γ].
 Proof.
 revert j n; induction x; intros.
-- now exists (rel_zero j).
-- now exists (rel_one j).
-- now exists (rel_eq j (n + i)).
+- now exists (Rel_zero j).
+- now exists (Rel_one j).
+- now exists (Rel_eq j (n + i)).
 - destruct (IHx1 0 (2 + n)) as [ϕ1 Hϕ1];
   destruct (IHx2 1 (2 + n)) as [ϕ2 Hϕ2].
-  exists ∃[∃[rel_add 0 1 (2 + j) ∧` ϕ1 ∧` ϕ2]].
+  exists ∃[∃[Rel_add 0 1 (2 + j) ∧` ϕ1 ∧` ϕ2]].
   simpl in *; split.
   + intros H. exists (eval (x2<<n) Γ), (eval (x1<<n) Γ).
     repeat split. easy.
@@ -239,9 +239,9 @@ revert j n; induction x; intros.
     rewrite ?eval_shift_vars; congruence.
 Defined.
 
-Lemma reduce_la_eq x y Γ :
-  Nat |= (la_eq x y)[Γ] <-> 
-  Nat |= (∃[la_eq #0 (x<<1) ∧` la_eq #0 (y<<1)])[Γ].
+Lemma reduce_LA_eq x y Γ :
+  Nat |= (LA_eq x y)[Γ] <-> 
+  Nat |= (∃[LA_eq #0 (x<<1) ∧` LA_eq #0 (y<<1)])[Γ].
 Proof.
 split; simpl.
 - intros H. exists (eval x Γ).
@@ -252,9 +252,9 @@ split; simpl.
   simpl in *; congruence.
 Qed.
 
-Lemma reduce_la_le x y Γ :
-  Nat |= (la_le x y)[Γ] <-> 
-  Nat |= (∃[∃[la_le #0 #1 ∧` la_eq #0 (x<<2) ∧` la_eq #1 (y<<2)]])[Γ].
+Lemma reduce_LA_le x y Γ :
+  Nat |= (LA_le x y)[Γ] <-> 
+  Nat |= (∃[∃[LA_le #0 #1 ∧` LA_eq #0 (x<<2) ∧` LA_eq #1 (y<<2)]])[Γ].
 Proof.
 split; simpl.
 - intros H; exists (eval y Γ), (eval x Γ); repeat split.
@@ -265,8 +265,8 @@ split; simpl.
   simpl in *; congruence.
 Qed.
 
-Lemma la_le_iff_rel_le i j Γ :
-  Nat |= (la_le #i #j)[Γ] <-> NatR |= (rel_le i j)[Γ].
+Lemma LA_le_iff_Rel_le i j Γ :
+  Nat |= (LA_le #i #j)[Γ] <-> NatR |= (Rel_le i j)[Γ].
 Proof.
 easy.
 Qed.
@@ -278,14 +278,14 @@ destruct a.
 - (* Equality relation. *)
   destruct reduce_la_term with (j:=0)(x:=x)(n:=1) as [ϕx Hx];
   destruct reduce_la_term with (j:=0)(x:=y)(n:=1) as [ϕy Hy].
-  eexists; symmetry; etransitivity. apply reduce_la_eq.
+  eexists; symmetry; etransitivity. apply reduce_LA_eq.
   apply Realizes_ex, Realizes_and; easy.
 - (* Less or equal relation. *)
   destruct reduce_la_term with (j:=0)(x:=x)(n:=2) as [ϕx Hx].
   destruct reduce_la_term with (j:=1)(x:=y)(n:=2) as [ϕy Hy].
-  eexists; symmetry; etransitivity. apply reduce_la_le.
+  eexists; symmetry; etransitivity. apply reduce_LA_le.
   apply Realizes_ex, Realizes_ex, Realizes_and.
-  apply la_le_iff_rel_le. apply Realizes_and; easy.
+  apply LA_le_iff_Rel_le. apply Realizes_and; easy.
 Defined.
 
 Corollary convert_formula_to_rformula φ :
